\documentclass[10pt]{article}
\usepackage{amsmath}
\title{CSCI 303, Homework 0 (Warm-up)}
\author{Nathan Owen}
\date{\today}

\begin{document}
\maketitle
\section{Problem One}

\begin{flushleft}
Prove by induction that $$\sum\limits_{i=1}^n i\cdot i! = (n+1)! - 1$$ for all $n \geq 1$. 
\end{flushleft}
\textit{Proof:}


\begin{flushleft}
\textbf{Base Case:} If $n=1$, then $(1\cdot 1!) = (1+1)!-1$ which simplifies to $1 = 1$
\end{flushleft}



\begin{flushleft}
\textbf{Inductive hypothesis:} For all $n\geq 1,$ $\sum\limits_{i=1}^n i\cdot i! = (n+1)! - 1$.
\end{flushleft}

\begin{flushleft}
\textbf{Inductive step:} Assume that the inductive hypothesis is true for $n$. We then need to prove that $\sum\limits_{i=1}^{n+1} i\cdot i! = ((n+1)+1)! - 1$. Because $\sum\limits_{i=1}^{n+1} i\cdot i!$ is $\sum\limits_{i=1}^n i\cdot i! + ((n+1)\cdot (n+1)!)$, the inductive hypothesis allows us to make the following substitution and then solve algebraically. 
\begin{align}
((n+1)+1)! - 1 &= \sum\limits_{i=1}^n i\cdot i! + ((n+1)\cdot (n+1)!)\\
&= ((n+1)! -1) + ((n+1)\cdot (n+1)!)\\
&=(n+1)! + (n+1)!(n+1) -1\\
&=(n+1)!(1+(n+1))-1\\
&=(n+1)!(n+2)-1\\
(n+2)!-1 &= (n+2)!-1
\end{align}

\end{flushleft}

\begin{flushleft}
\textbf{Conclusion:} By the principle of induction, the inductive hypothesis is true for all $n \geq 1$
\end{flushleft}




\section{Problem Two}

\begin{flushleft}
Prove by induction that $$\sum\limits_{i=1}^n \frac{1}{i^2}\leq 2- \frac{1}{n}$$ for all $n \geq 1$. 
\end{flushleft}
\textit{Proof:}


\begin{flushleft}
\textbf{Base Case:} If $n=1$, then $\frac{1}{1^2}  \leq 2 - \frac{1}{1}$ which simplifies to $1 \leq 1$
\end{flushleft}



\begin{flushleft}
\textbf{Inductive hypothesis:} For all $n\geq 1,$ $\sum\limits_{i=1}^n \frac{1}{i^2}\leq 2- \frac{1}{n}$.
\end{flushleft}

\begin{flushleft}
\textbf{Inductive step:} Assume that the inductive hypothesis is true for $n$. We then need to prove that $\sum\limits_{i=1}^{n+1} \frac{1}{i^2}\leq 2- \frac{1}{n+1}$. Because $\sum\limits_{i=1}^{n+1} \frac{1}{i^2}$ is $\sum\limits_{i=1}^n \frac{1}{i^2} + \frac{1}{(n+1)^2}$, and by the induction hypothesis, $\sum\limits_{i=1}^n \frac{1}{i^2}\leq 2- \frac{1}{n}$, then if we substitute $\sum\limits_{i=1}^n \frac{1}{i^2}$ with $2- \frac{1}{n}$ and the resulting inequality is algebraically true, we know that $\sum\limits_{i=1}^{n+1} \frac{1}{i^2}\leq 2- \frac{1}{n+1}$ is also true because the original term is less than or equal to that which is being substituted. And so,
\begin{align}
(2- \frac{1}{n}) + \frac{1}{(n+1)^2} &\leq 2- \frac{1}{n+1}\\
\frac{1}{(n+1)^2} - \frac{1}{n} &\leq -\frac{1}{n+1} \\
\frac{1}{(n+1)^2} &\leq \frac{1}{n} -\frac{1}{n+1} \\
1 &\leq \frac{(n+1)^2}{n} -(n+1)\\
1 &\leq \frac{n^2+2n+1}{n}-n-1\\
1 &\leq n+2+\frac{1}{n} -n-1\\
1 &\leq 1+\frac{1}{n}
\end{align}

\end{flushleft}

\begin{flushleft}
\textbf{Conclusion:} By the principle of induction, the inductive hypothesis is true for all $n \geq 1$
\end{flushleft}

\begin{flushleft}

\end{flushleft}


\end{document}